src/Cat.v
@@ -12,6 +12,10 @@ Require Import Category.Lib.
 Require Import Category.Theory.Category.
 Require Import Category.Structure.BiCCC.
 
+Set Implicit Arguments.
+Unset Strict Implicit.
+Unset Printing Implicit Defensive.
+
 Set Equations With UIP.
 
 Generalizable All Variables.
