src/Eval.v
@@ -11,9 +11,14 @@ Require Import
   Pact.Lang
   Pact.SemExp.
 
+Set Implicit Arguments.
+Unset Strict Implicit.
+Unset Printing Implicit Defensive.
+
 Set Equations With UIP.
 
 Generalizable All Variables.
+Set Primitive Projections.
 
 Import ListNotations.
 
