src/Exp.v
@@ -3,11 +3,14 @@ Require Import
   Pact.Lib
   Pact.Ty.
 
+Set Implicit Arguments.
+Unset Strict Implicit.
+Unset Printing Implicit Defensive.
+
 Set Equations With UIP.
 
 Generalizable All Variables.
-
-Section Exp.
+Set Primitive Projections.
 
 Import ListNotations.
 
@@ -99,65 +102,43 @@ Derive Signature NoConfusionHom Subterm for Exp.
 
 Fixpoint Exp_size {Γ τ} (e : Exp Γ τ) : nat :=
   match e with
-  | VAR _ v     => 1
-  | LAM _ e     => 1 + Exp_size e
-  | APP _ e1 e2 => 1 + Exp_size e1 + Exp_size e2
+  | VAR v     => 1
+  | LAM e     => 1 + Exp_size e
+  | APP e1 e2 => 1 + Exp_size e1 + Exp_size e2
 
-  | Error _ _   => 1
-  | Lit _ _     => 1
-  | Bltn _ _    => 1
-  | Symbol _ _  => 1
-  | If _ b t e  => 1 + Exp_size b + Exp_size t + Exp_size e
-  | Pair _ x y  => 1 + Exp_size x + Exp_size y
-  | Fst _ p     => 1 + Exp_size p
-  | Snd _ p     => 1 + Exp_size p
-  | Nil _       => 1
-  | Cons _ x xs => 1 + Exp_size x + Exp_size xs
-  | Car _ xs    => 1 + Exp_size xs
-  | Cdr _ xs    => 1 + Exp_size xs
-  | IsNil _ xs  => 1 + Exp_size xs
-  | Seq _ x y   => 1 + Exp_size x + Exp_size y
+  | Error _ _  => 1
+  | Lit _ _    => 1
+  | Bltn _ _   => 1
+  | Symbol _ _ => 1
+  | If b t e   => 1 + Exp_size b + Exp_size t + Exp_size e
+  | Pair x y   => 1 + Exp_size x + Exp_size y
+  | Fst p      => 1 + Exp_size p
+  | Snd p      => 1 + Exp_size p
+  | Nil _      => 1
+  | Cons x xs  => 1 + Exp_size x + Exp_size xs
+  | Car xs     => 1 + Exp_size xs
+  | Cdr xs     => 1 + Exp_size xs
+  | IsNil xs   => 1 + Exp_size xs
+  | Seq x y    => 1 + Exp_size x + Exp_size y
 
-  | Capability _ _ _ n p v => 1 + Exp_size n + Exp_size p + Exp_size v
-  | WithCapability _ _ nm p m c e =>
+  | Capability _ _ n p v => 1 + Exp_size n + Exp_size p + Exp_size v
+  | WithCapability _ nm p m c e =>
       1 + Exp_size nm + Exp_size p + Exp_size m + Exp_size c + Exp_size e
-  | ComposeCapability _ _ nm p m c =>
+  | ComposeCapability _ nm p m c =>
       1 + Exp_size nm + Exp_size p + Exp_size m + Exp_size c
-  | InstallCapability _ c => 1 + Exp_size c
-  | RequireCapability _ c => 1 + Exp_size c
+  | InstallCapability c => 1 + Exp_size c
+  | RequireCapability c => 1 + Exp_size c
   end.
 
 Corollary Exp_size_preserved {Γ τ} (e1 e2 : Exp Γ τ) :
   Exp_size e1 ≠ Exp_size e2 → e1 ≠ e2.
 Proof. repeat intro; subst; contradiction. Qed.
 
-End Exp.
-
-Arguments ZV {_ _}.
-Arguments SV {_ _ _} _.
-
-Arguments VAR {Γ τ} _.
-Arguments LAM {Γ dom cod} _.
-Arguments APP {Γ dom cod} _ _.
 Arguments Error {Γ τ} _.
 Arguments Lit {Γ ty} _.
 Arguments Bltn {Γ τ} _.
 Arguments Symbol {Γ} _.
-Arguments If {Γ τ} _ _ _.
-Arguments Pair {Γ τ1 τ2} _ _.
-Arguments Fst {Γ τ1 τ2} _.
-Arguments Snd {Γ τ1 τ2} _.
 Arguments Nil {Γ τ}.
-Arguments Cons {Γ τ} _ _.
-Arguments Car {Γ τ} _.
-Arguments Cdr {Γ τ} _.
-Arguments IsNil {Γ τ} _.
-Arguments Seq {Γ τ τ'} _ _.
-Arguments Capability {_ p v} _ _ _.
-Arguments WithCapability {_ p v τ} _ _ _ _ _ _.
-Arguments ComposeCapability {_ p v} _ _ _ _ _.
-Arguments InstallCapability {_ p v} _.
-Arguments RequireCapability {_ p v} _.
 
 Declare Scope Var_scope.
 Bind Scope Var_scope with Var.
