src/Log.v
@@ -6,9 +6,14 @@ Require Import
   Pact.Exp
   Pact.Sub.
 
+Set Implicit Arguments.
+Unset Strict Implicit.
+Unset Printing Implicit Defensive.
+
 Set Equations With UIP.
 
 Generalizable All Variables.
+Set Primitive Projections.
 
 Section Log.
 
