src/SemExp.v
@@ -13,11 +13,14 @@ Require Import
   Pact.Lang
   Pact.Lang.Capability.
 
+Set Implicit Arguments.
+Unset Strict Implicit.
+Unset Printing Implicit Defensive.
+
 Set Equations With UIP.
 
 Generalizable All Variables.
-
-Section SemExp.
+Set Primitive Projections.
 
 Import ListNotations.
 
@@ -254,7 +257,5 @@ Proof.
     unfold RWSE_join.
     reflexivity.
 Abort.
-
-End SemExp.
 
 Notation "f =<< x" := (x >>= f) (at level 42, right associativity).
